Pull field element length into felem
The main changes are in Field.v. Extract the length of the word list
representing a field element in memory from the Bignum hidden inside
FElem over to the felem type. That way, one does not need to fiddle with
separation logic everytime the length of that list is needed.

There are a few helper lemmas for conversions between the different
ways to represent field elements in memory in Field.v, and two new
tactics to automatically rewrite between the types.

Use those new tactics throughout existing proofs, and get rid of some of
the convolution the Bignum type was causing.

src/Bedrock/Field/Interface/Compilation2.v
@@ -1,5 +1,6 @@
 Require Import Rupicola.Lib.Api.
 Require Import Rupicola.Lib.Alloc.
+Require Import coqutil.Macros.symmetry.
 Require Import Crypto.Bedrock.Specs.Field.
 Require Import Crypto.Arithmetic.PrimeFieldTheorems.
 Local Open Scope Z_scope.
@@ -24,7 +25,7 @@ Section Compile.
 
   (* TODO: Replace uses of the old FElem with this? *)
   Definition FElem mbounds ptr v :=
-    (Lift1Prop.ex1 (fun v' => (emp (feval v' = v /\ maybe_bounded mbounds v') * FElem ptr v')%sep)).
+    (Lift1Prop.ex1 (fun v' : felem => (emp (feval v' = v /\ maybe_bounded mbounds v') * FElem ptr v')%sep)).
 
   Lemma drop_bounds_FElem x_ptr x bounds
     : Lift1Prop.impl1 (FElem bounds x_ptr x)
@@ -48,38 +49,6 @@ Section Compile.
     sepsimpl; simpl in *; eauto using relax_bounds.
   Qed.
 
-  Lemma FElem'_iff_bytes
-    : forall px : word.rep,
-      Lift1Prop.iff1 (Lift1Prop.ex1 (Placeholder px)) (Lift1Prop.ex1 (FElem None px)).
-  Proof using field_representation_ok mem_ok word_ok.
-    unfold FElem.
-    intros.
-    split; intros.
-    {
-      destruct H as [bs H].
-      apply Placeholder_impl_FElem_bytes in H.
-      do 2 eexists.
-      sepsimpl; simpl; eauto.
-    }
-    {
-      destruct H as [ws [? H]].
-      sepsimpl.
-      eexists.
-      eapply FElem_impl_Placeholder; eauto.
-    }
-  Qed.
-
-  Lemma FElem'_to_bytes
-    : forall bounds px x,
-      Lift1Prop.impl1 (FElem bounds px x) (Lift1Prop.ex1 (Placeholder px)).
-  Proof.
-    intros. cbv [FElem]. intros m [f F].
-    extract_ex1_and_emp_in F.
-    sepsimpl.
-    eexists. eapply FElem_impl_Placeholder.
-    eassumption.
-  Qed.
-
   #[refine]
    Instance felem_alloc : Allocable (FElem None) :=
     {|
@@ -88,21 +57,27 @@ Section Compile.
     |}.
   Proof.
     {
+      pose proof Types.word_size_in_bytes_pos as HT.
       intros; intros m H.
-      apply FElem'_to_bytes in H.
-      cbv[Placeholder] in *.
-      sepsimpl.
-      eexists.
-      pose felem_size_ok.
-      ssplit; try eassumption.
-      lia.
+      cbv [FElem anybytes] in *. sepsimpl.
+      seprewrite_in felem_to_bytes H0.
+      eexists; ssplit; sepsimpl. use_sep_assumption. cancel.
+      cancel_seps_at_indices 0%nat 0%nat. reflexivity. cancel.
+      rewrite ws2bs_felem_length; trivial.
+      cbv [felem_size_in_bytes]. lia.
+      apply ws2bs_felem_width.
     }
     {
       intros; intros m H.
-      apply FElem'_iff_bytes.
-      cbv [Memory.anybytes Placeholder] in *. sepsimpl.
-      eexists; try eassumption.
-      sepsimpl; try eassumption.
+      cbv [FElem anybytes] in *. sepsimpl.
+      eexists. eexists. sepsimpl.
+      3: {
+        SeparationLogic.seprewrite (symmetry! (felem_from_bytes px x)).
+        lia.
+        sepsimpl. rewrite H. reflexivity. trivial.
+      }
+      reflexivity.
+      cbv [maybe_bounded]. trivial.
     }
   Defined.
 
@@ -157,6 +132,7 @@ Section Compile.
     unfold FElem in *.
     sepsimpl.
     prove_field_compilation.
+    rewrite ws2bs_felem_length. lia.
     apply H6.
 
     eapply Proper_sep_impl1; eauto.
@@ -202,6 +178,7 @@ Section Compile.
     unfold FElem in *.
     sepsimpl.
     prove_field_compilation.
+    rewrite ws2bs_felem_length. lia.
     apply H4.
 
     eapply Proper_sep_impl1; eauto.
@@ -282,6 +259,7 @@ Section Compile.
     unfold FElem in *.
     sepsimpl.
     prove_field_compilation.
+    rewrite ws2bs_felem_length. lia.
     apply H3.
 
     extract_ex1_and_emp_in_goal; ssplit; eauto.
@@ -324,6 +302,7 @@ Section Compile.
     unfold FElem in *.
     extract_ex1_and_emp_in H1.
     prove_field_compilation.
+    rewrite ws2bs_felem_length. lia.
     match goal with H : _ |- _ => rewrite word.of_Z_unsigned in H end.
     apply H3.
     extract_ex1_and_emp_in_goal; ssplit; eauto.
