src/Bedrock/Specs/Field.v
@@ -1,11 +1,15 @@
+Require Import Bedrock.Field.Common.Types.
 Require Import coqutil.Byte coqutil.Word.LittleEndianList.
-Require Import Rupicola.Lib.Api.
+From coqutil.Macros Require Import symmetry.
 Require Import Crypto.Algebra.Hierarchy.
 Require Import Crypto.Arithmetic.PrimeFieldTheorems.
 Require Import Crypto.Bedrock.Field.Synthesis.Generic.Bignum.
 Require Import Crypto.Bedrock.Field.Common.Arrays.MaxBounds.
 Require Import Crypto.COperationSpecifications.
 Require Import Crypto.Util.ZUtil.ModInv.
+Require Import Rupicola.Lib.Api.
+Require Rupicola.Lib.Arrays.
+
 Local Open Scope Z_scope.
 Import bedrock2.Memory.
 
@@ -36,17 +40,18 @@ Class FieldRepresentation
       {field_parameters : FieldParameters}
       {width: Z} {BW: Bitwidth width} {word: word.word width} {mem: map.map word Byte.byte}
        :=
-  { felem := list word;
-    feval : felem -> F M_pos;
+  { felem_size_in_words : nat;
+    felem := {x : list word | length x = felem_size_in_words};
+    feval : list word -> F M_pos;
 
     feval_bytes : list byte -> F M_pos;
-    felem_size_in_words : nat;
-    felem_size_in_bytes : Z := Z.of_nat felem_size_in_words * bytes_per_word width; (* for stack allocation *)
+    felem_size_in_bytes : Z := (Z.of_nat felem_size_in_words) * bytes_per_word width; (* for stack allocation *)
     encoded_felem_size_in_bytes : nat; (* number of bytes when serialized *)
     bytes_in_bounds : list byte -> Prop;
 
     (* Memory layout *)
-    FElem : word -> list word -> mem -> Prop := Bignum felem_size_in_words;
+    FElem : word -> felem -> mem -> Prop := fun px x =>
+      (array scalar (word.of_Z (bytes_per_word width)) px (proj1_sig x));
     FElemBytes : word -> list byte -> mem -> Prop :=
       fun addr bs =>
         (emp (length bs = encoded_felem_size_in_bytes
@@ -54,28 +59,10 @@ Class FieldRepresentation
          * array ptsto (word.of_Z 1) addr bs)%sep;
 
     bounds : Type;
-    bounded_by : bounds -> felem -> Prop;
+    bounded_by : bounds -> list word -> Prop;
     (* for saturated implementations, loose/tight bounds are the same *)
     loose_bounds : bounds;
     tight_bounds : bounds;
-  }.
-
-Definition Placeholder
-        {field_parameters : FieldParameters}
-        {width: Z} {BW: Bitwidth width} {word: word.word width} {mem: map.map word Byte.byte}
-        {field_representation : FieldRepresentation(mem:=mem)}
-        (p : word) (bs : list byte): mem -> Prop :=
-(sep (map.of_list_word_at p bs)
-  (emp (Z.of_nat (length bs) = felem_size_in_bytes))).
-
-Class FieldRepresentation_ok
-      {field_parameters : FieldParameters}
-      {width: Z} {BW: Bitwidth width} {word: word.word width} {mem: map.map word Byte.byte}
-      {field_representation : FieldRepresentation} := {
-    relax_bounds :
-      forall X : felem, bounded_by tight_bounds X
-                        -> bounded_by loose_bounds X;
-    felem_size_ok : felem_size_in_bytes <= 2^width
   }.
 
 Section FunctionSpecs.
@@ -95,15 +82,21 @@ Section FunctionSpecs.
 
   Import WeakestPrecondition.
 
+  #[warnings="-uniform-inheritance", global]
+  Coercion felem_to_list (x : felem) : list word := proj1_sig x.
+
+  #[local] Coercion Z.to_nat : Z >-> nat.
+
   Definition unop_spec {name} (op: UnOp name) :=
     fnspec! name (pout px : word) / (x : felem) out Rr,
     { requires tr mem :=
         bounded_by un_xbounds x
+        /\ length out = felem_size_in_bytes
         /\ (exists Ra, (FElem px x * Ra)%sep mem)
-        /\ (Placeholder pout out * Rr)%sep mem;
+        /\ (out$@pout * Rr)%sep mem;
       ensures tr' mem' :=
         tr = tr' /\
-        exists out,
+        exists out : felem,
           feval out = un_model (feval x)
           /\ bounded_by un_outbounds out
           /\ (FElem pout out * Rr)%sep mem' }.
@@ -122,12 +115,13 @@ Section FunctionSpecs.
     { requires tr mem :=
         bounded_by bin_xbounds x
         /\ bounded_by bin_ybounds y
+        /\ length out = felem_size_in_bytes
         /\ (exists Rx, (FElem px x * Rx)%sep mem)
         /\ (exists Ry, (FElem py y * Ry)%sep mem)
-        /\ (Placeholder pout out * Rr)%sep mem;
+        /\ (out$@pout * Rr)%sep mem;
       ensures tr' mem' :=
         tr = tr' /\
-        exists out,
+        exists out : felem,
           feval out = bin_model (feval x) (feval y)
           /\ bounded_by bin_outbounds out
           /\ (FElem pout out * Rr)%sep mem' }.
@@ -158,11 +152,12 @@ Section FunctionSpecs.
     fnspec! from_bytes (pout px : word) / (out bs : list byte) Rr,
     { requires tr mem :=
         (exists Ra, (array ptsto (word.of_Z 1) px bs * Ra)%sep mem)
-        /\ (Placeholder pout out * Rr)%sep mem
+        /\ (out$@pout * Rr)%sep mem
+        /\ length out = felem_size_in_bytes
         /\ Field.bytes_in_bounds bs;
       ensures tr' mem' :=
         tr = tr' /\
-        exists X, feval X = feval_bytes bs
+        exists X : felem, feval X = feval_bytes bs
              /\ bounded_by tight_bounds X
              /\ (FElem pout X * Rr)%sep mem' }.
 
@@ -181,7 +176,8 @@ Section FunctionSpecs.
   Instance spec_of_felem_copy : spec_of felem_copy :=
     fnspec! felem_copy (pout px : word) / (x : felem) out R,
     { requires tr mem :=
-        (FElem px x * Placeholder pout out * R)%sep mem;
+        (FElem px x * out$@pout * R)%sep mem /\
+        length out = felem_size_in_bytes;
       ensures tr' mem' :=
         tr = tr' /\
         (FElem px x * FElem pout x * R)%sep mem' }.
@@ -189,10 +185,11 @@ Section FunctionSpecs.
   Instance spec_of_from_word : spec_of from_word :=
     fnspec! from_word (pout x : word) / out R,
     { requires tr mem :=
-        (Placeholder pout out * R)%sep mem;
+        (out$@pout * R)%sep mem /\
+        length out = felem_size_in_bytes;
       ensures tr' mem' :=
         tr = tr' /\
-        exists X, feval X = F.of_Z _ (word.unsigned x)
+        exists X : felem, feval X = F.of_Z _ (word.unsigned x)
              /\ bounded_by tight_bounds X
              /\ (FElem pout X * R)%sep mem' }.
 
@@ -202,9 +199,10 @@ Section FunctionSpecs.
     fnspec! select_znz (pout pc px py : word) / out Rout Rx Ry x y,
     {
         requires tr mem :=
-        (Placeholder pout out * Rout)%sep mem /\
+        (out$@pout * Rout)%sep mem /\
         (FElem px x * Rx)%sep mem /\
         (FElem py y * Ry)%sep mem /\
+        length out = felem_size_in_bytes /\
         ZRange.is_bounded_by_bool (word.unsigned pc) bit_range = true;
         ensures tr' mem' :=
         if ((word.unsigned pc) =? 1)
@@ -232,6 +230,16 @@ End FunctionSpecs.
 Existing Instances spec_of_UnOp spec_of_BinOp bin_mul un_square bin_add bin_sub
          un_scmula24 un_inv spec_of_felem_copy spec_of_from_word.
 
+Class FieldRepresentation_ok
+      {field_parameters : FieldParameters}
+      {width: Z} {BW: Bitwidth width} {word: word.word width} {mem: map.map word Byte.byte}
+      {field_representation : FieldRepresentation} := {
+    relax_bounds :
+      forall X : felem, bounded_by tight_bounds X
+                        -> bounded_by loose_bounds X;
+    felem_size_ok : felem_size_in_bytes <= 2^width
+  }.
+
 Section SpecProperties.
   Context {width: Z} {BW: Bitwidth width} {word: word.word width} {mem: map.map word Byte.byte}.
   Context {locals: map.map String.string word}.
@@ -241,102 +249,318 @@ Section SpecProperties.
   Context {ext_spec_ok : Semantics.ext_spec.ok ext_spec}.
   Context {field_parameters : FieldParameters}
           {field_representation : FieldRepresentation}
-          {field_representation_ok : FieldRepresentation_ok}.
+          {field_representation_ok : FieldRepresentation_ok}.    
 
-  Lemma felem_size_in_bytes_mod :
-         felem_size_in_bytes mod Memory.bytes_per_word width = 0.
-  Proof. apply Z_mod_mult. Qed.
+  #[local] Coercion Z.to_nat : Z >-> nat.
 
-  Local Coercion Z.to_nat : Z >-> nat.
-
-  Lemma Placeholder_impl_FElem_bytes p bs :
-    Lift1Prop.impl1 (Placeholder p bs) (FElem p (bs2ws (bytes_per_word width) bs)).
+  #[local] Notation ws2bs := (ws2bs (width:=width)).
+  #[local] Notation bs2ws := (bs2ws (width:=width)).
+  #[local] Notation bytes_per := (bytes_per (width:=width)).
+  
+  Lemma felem_length (x : felem) : length (felem_to_list x) = felem_size_in_words.
   Proof.
-    repeat intro.
-    pose (Bignum_of_bytes felem_size_in_words p bs) as HBignum.
-    epose (array1_iff_eq_of_list_word_at p bs) as HArray.
-    pose felem_size_ok.
-    cbv [FElem Placeholder felem_size_in_bytes] in *.
-    intros.
-    extract_ex1_and_emp_in_hyps. apply HBignum. lia.
-      apply HArray. lia. assumption.
+    cbv [felem_to_list]. destruct x. trivial.
   Qed.
 
-  Lemma FElem_impl_Placeholder p ws :
-    Lift1Prop.impl1 (FElem p ws) (Placeholder p (ws2bs (bytes_per_word width) ws)).
+  (* nat equality is decidable, which means that all length proofs are equal and field
+   elements are equal if their underlying lists are equal. *)
+  Lemma eq_felem {x y : felem} : proj1_sig x = proj1_sig y -> x = y.
   Proof.
-    repeat intro.
-    pose (Bignum_to_bytes felem_size_in_words p ws) as HBignum.
-    pose felem_size_ok.
-    cbv [FElem Placeholder felem_size_in_bytes] in *.
-    apply HBignum in H. extract_ex1_and_emp_in_hyps.
-    extract_ex1_and_emp_in_goal; split.
-    apply array1_iff_eq_of_list_word_at; try assumption.
-    lia.
-    pose Types.word_size_in_bytes_pos.
-    lia.
+    destruct x as [x px], y as [y py].
+    cbv [proj1_sig]. intro. subst.
+    apply f_equal,  Eqdep_dec.UIP_dec. eapply Nat.eq_dec.
   Qed.
 
-  Lemma Placeholder_iff_FElem_bytes p bs : 
-    Lift1Prop.iff1 (Placeholder p bs) (sep (FElem p ((bs2ws (bytes_per_word width) bs))) (emp (Datatypes.length bs = felem_size_in_bytes))).
+  Lemma bytes_per_as_Z : bytes_per access_size.word = bytes_per_word width.
   Proof.
-    repeat intro.
-    pose (Bignum_of_bytes felem_size_in_words p bs) as HBignum.
-    epose (array1_iff_eq_of_list_word_at p bs) as HArray.
-    pose felem_size_ok.
-    cbv [FElem Placeholder felem_size_in_bytes] in *.
-    split; intros.
-    - sepsimpl. apply HBignum. lia.
-      apply HArray. lia. assumption.
-      lia.
-    - sepsimpl. apply HArray; try lia. apply HBignum; try lia.
-      assumption. pose Types.word_size_in_bytes_pos. lia.
+    cbv [bytes_per_word bytes_per] in *; lia.
+  Qed.
+  Lemma bytes_per_of_nat_to_nat_id : Z.of_nat (bytes_per_word width) = bytes_per_word width.
+  Proof.
+    pose word_size_in_bytes_pos; lia.
+  Qed.
+  Lemma of_nat_bytes_per: (Z.of_nat (bytes_per access_size.word)) = bytes_per_word width.
+  Proof.
+    rewrite bytes_per_as_Z, bytes_per_of_nat_to_nat_id. exact eq_refl.
   Qed.
 
-  Lemma Placeholder_iff_FElem_words p ws :
-    Lift1Prop.iff1 (sep (Placeholder p (ws2bs (bytes_per_word width) ws)) (emp (Datatypes.length ws = felem_size_in_words))) (FElem p ws).
-  Proof.
-    repeat intro.
-    pose (Bignum_to_bytes felem_size_in_words p ws) as HBignum.
-    pose felem_size_ok.
-    cbv [FElem Placeholder felem_size_in_bytes] in *.
-    split; intros.
-    - sepsimpl. apply HBignum.
-      sepsimpl; try lia.
-      apply array1_iff_eq_of_list_word_at; try assumption; try lia.
-    - apply HBignum in H. sepsimpl.
-      apply array1_iff_eq_of_list_word_at; try assumption; lia.
-      rewrite H. pose Types.word_size_in_bytes_pos. lia.
-      pose Types.word_size_in_bytes_pos.
-      rewrite ws2bs_length in H. nia.
+  Lemma felem_size_in_bytes_mod : felem_size_in_bytes mod bytes_per_word width = 0.
+  Proof. 
+    apply Z_mod_mult.
   Qed.
 
-  (* this is almost bytearray_iff_bytes *)
-  Lemma Placeholder_iff_array1 p bs :
-    Datatypes.length bs = felem_size_in_bytes ->
-    Lift1Prop.iff1 (Placeholder p bs) (array ptsto (word.of_Z 1) p bs).
-  Proof.
-    repeat intro.
-    cbv [Placeholder].
-    pose felem_size_ok. apply iff1_sym.
-    rewrite array1_iff_eq_of_list_word_at; try assumption.
-    - split; intros; extract_ex1_and_emp_in_goal; extract_ex1_and_emp_in_hyps; try split; try assumption.
-      rewrite H. pose Types.word_size_in_bytes_pos. cbv [felem_size_in_bytes]. lia.
-    - lia.
+  Lemma felem_size_in_bytes_mod_nat :
+    (felem_size_in_bytes mod (bytes_per_word width) = 0)%nat.
+  Proof. 
+    pose proof word_size_in_bytes_pos.
+    cbv [bytes_per_word bytes_per felem_size_in_bytes] in *.
+    rewrite Modulo.Z.mod_to_nat; try lia.
+    rewrite Z_mod_mult. lia.
   Qed.
 
+  Lemma ws2bs_felem_length (x : felem):
+    length (ws2bs (bytes_per_word width) x) = felem_size_in_bytes.
+  Proof.
+    rewrite ws2bs_length, felem_length.
+    cbv [bytes_per_word felem_size_in_bytes] in *. lia.
+  Qed.
+
+  Lemma ws2bs_felem_width (x : felem):
+    Z.of_nat (length (ws2bs (bytes_per_word width) x)) <= 2 ^ width.
+  Proof.
+    destruct x. pose felem_size_ok.
+    cbv [felem_size_in_bytes bytes_per_word bytes_per felem_to_list proj1_sig] in *.
+    rewrite ws2bs_length. lia.
+  Qed.
+
+  Lemma bs2ws_felem_length bs : 
+    length bs = felem_size_in_bytes ->
+    length (bs2ws (bytes_per_word width) bs) = felem_size_in_words.
+  Proof.
+    intros H.
+    pose proof felem_size_ok.
+    pose proof word_size_in_bytes_pos.
+    pose proof felem_size_in_bytes_mod.
+    cbv [felem_size_in_bytes] in *. rewrite bs2ws_length; try ZnWords; try lia.
+    rewrite H, <- Z2Nat.inj_div; try lia.
+    rewrite Z_div_mult; try lia. (* TODO without div_mult neither lia nor ZnWords can solve this, expected? *)
+    rewrite H.
+    rewrite Modulo.Z.mod_to_nat; try lia. (* TODO without mod_to_nat neither lia nor ZnWords can solve this, expected?  *)
+  Qed.
+
+  Definition ws2felem (ws : list word) : felem.
+  Proof.
+    refine (exist _ (if (length ws =? felem_size_in_words)%nat then 
+      (ws) else 
+      (List.repeat (word.of_Z 0) felem_size_in_words)) _).
+    abstract (rewrite NatUtil.beq_nat_eq_nat_dec;
+    destruct (Nat.eq_dec (length ws) (felem_size_in_words));
+    [ assumption | apply repeat_length]).
+  Defined.
+
+  Lemma felem_to_list_ws2felem (ws : list word) :
+    length ws = felem_size_in_words ->
+    felem_to_list (ws2felem ws) = ws.
+  Proof.
+    intros H. cbv [ws2felem felem_to_list proj1_sig].
+    rewrite H.
+    rewrite Nat.eqb_refl.
+    exact eq_refl.
+  Qed.
+
+  Lemma ws2felem_felem_to_list (x : felem) :
+    ws2felem (felem_to_list x) = x.
+  Proof.
+    apply eq_felem.
+    pose proof felem_length as H.
+    cbv [ws2felem proj1_sig].
+    rewrite H.
+    rewrite Nat.eqb_refl.
+    exact eq_refl.
+  Qed.
+
+  Lemma felem_to_bytes p x :
+    Lift1Prop.iff1 (FElem p x) ((ws2bs (bytes_per_word width) x)$@p).
+  Proof.
+    cbv [FElem].
+    
+    epose proof ((bytes_of_words _ _)) as Hbytes_of_words.
+    cbn [id] in Hbytes_of_words.
+    rewrite of_nat_bytes_per in *.
+
+    etransitivity. exact Hbytes_of_words.
+    exact (array1_iff_eq_of_list_word_at _ _ (ws2bs_felem_width _)).
+  Qed.
+
+  Lemma felem_to_bytearray p x :
+    Lift1Prop.iff1 (FElem p x) (array ptsto (word.of_Z 1) p (ws2bs (bytes_per_word width) x)).
+  Proof.
+    etransitivity. exact (felem_to_bytes _ _).
+    exact (iff1_sym (array1_iff_eq_of_list_word_at _ _ (ws2bs_felem_width _))).
+  Qed.
+
+  Definition bs2felem (bs : list byte) : felem.
+  Proof.
+    refine (exist _ (if (length bs =? felem_size_in_bytes)%nat then 
+      ((bs2ws (bytes_per_word width) bs)) else 
+      (List.repeat (word.of_Z 0) felem_size_in_words)) _).
+    abstract (rewrite NatUtil.beq_nat_eq_nat_dec;
+    destruct (Nat.eq_dec (length bs) (felem_size_in_bytes));
+    [apply bs2ws_felem_length; assumption | apply repeat_length]).
+  Defined.
+
+  Lemma proj_bs2felem (bs : list byte) :
+    length bs = felem_size_in_bytes ->
+    proj1_sig (bs2felem bs) = (bs2ws (bytes_per_word width) bs).
+  Proof.
+    intros H.
+    cbv [bs2felem proj1_sig].
+    rewrite H.
+    rewrite Nat.eqb_refl.
+    exact eq_refl.
+  Qed.
+
+  Lemma felem_to_list_bs2felem (bs : list byte) :
+    length bs = felem_size_in_bytes ->
+    (felem_to_list (bs2felem bs)) = (bs2ws (bytes_per_word width) bs).
+  Proof.
+    intros H.
+    cbv [felem_to_list].
+    rapply proj_bs2felem.
+    assumption.
+  Qed.
+  
+  Lemma felem_from_bytes p bs :
+    length bs = felem_size_in_bytes ->
+    Lift1Prop.iff1 (bs$@p) (FElem p (bs2felem bs)).
+  Proof.
+    intros HL.
+    symmetry. etransitivity.
+    cbv [FElem]. 
+    rewrite proj_bs2felem; [|assumption].
+
+    epose proof ((words_of_bytes _ _)) as Hwords_of_bytes.
+    cbv [id] in Hwords_of_bytes.
+    rewrite of_nat_bytes_per in Hwords_of_bytes.
+    symmetry. rapply Hwords_of_bytes.
+    rewrite HL. rewrite bytes_per_as_Z. apply felem_size_in_bytes_mod_nat.
+
+    apply (array1_iff_eq_of_list_word_at _ _).
+    rewrite HL. pose proof felem_size_ok. lia.
+  Qed.
+
+  Lemma felem_from_bytearray p bs :
+    length bs = felem_size_in_bytes ->
+    Lift1Prop.iff1 (array ptsto (word.of_Z 1) p bs) (FElem p (bs2felem bs)).
+  Proof.
+    intros HL.
+
+    etransitivity.
+
+    apply array1_iff_eq_of_list_word_at.
+    assumption.
+    rewrite HL. pose proof felem_size_ok. lia.
+
+    apply felem_from_bytes.
+    assumption. 
+  Qed.
+
+  Lemma felem_to_Z_array p x :
+    Lift1Prop.iff1
+      (FElem p x)
+      (Array.array
+              (truncated_scalar access_size.word)
+              (word.of_Z (bytes_per_word width))
+              p (List.map word.unsigned x)).
+  Proof.
+    pose proof word_size_in_bytes_pos. 
+    cbv [FElem].
+    rewrite Util.array_truncated_scalar_scalar_iff1.
+    split; intros; sepsimpl; try assumption.
+  Qed.
+
+  Lemma FElemBytes_to_Z_array p bs :
+    Lift1Prop.iff1
+      (FElemBytes p bs)
+      (sep (map:=mem)
+           (emp (map:=mem)
+                (length bs = encoded_felem_size_in_bytes
+                 /\ bytes_in_bounds bs))
+           (Array.array
+              (Scalars.truncated_scalar access_size.one)
+              (word.of_Z 1) p (List.map byte.unsigned bs))).
+  Proof.
+    cbv [FElemBytes].
+    rewrite Util.array_truncated_scalar_ptsto_iff1.
+    rewrite ByteBounds.byte_map_of_Z_unsigned.
+    reflexivity.
+  Qed.
   Lemma M_nonzero : M <> 0.
   Proof. cbv [M]. congruence. Qed.
+
+  (* Rupicola Array helper lemmas.*)
+
+  Lemma FElem_as_array
+    : Field.FElem = Arrays.listarray_value access_size.word.
+  Proof.
+    unfold Field.FElem, Arrays.listarray_value.
+    simpl.
+    rewrite Z2Nat.id.
+    reflexivity.
+    pose word_size_in_bytes_pos.
+    lia.
+  Qed.
+    
+  Lemma felem_to_sizedlistarray p x :
+    Lift1Prop.iff1
+      (FElem p x)
+      (Arrays.sizedlistarray_value access_size.word felem_size_in_words p
+        (felem_to_list x)).
+  Proof.
+    rewrite FElem_as_array.
+    pose proof (felem_length x).
+    unfold Arrays.sizedlistarray_value.
+    split.
+    - intros. extract_ex1_and_emp_in_goal. split; assumption. 
+    - intros. extract_ex1_and_emp_in_hyps. assumption.
+  Qed. 
+
+  Lemma sizedlistarray_to_felem p x :
+    Datatypes.length x = felem_size_in_words ->
+    Lift1Prop.iff1 
+      (Arrays.sizedlistarray_value access_size.word felem_size_in_words p x)
+      (FElem p (ws2felem x)).
+  Proof.
+    split; intros.
+    SeparationLogic.seprewrite felem_to_sizedlistarray.
+    rewrite felem_to_list_ws2felem; [|assumption].
+    ecancel_assumption.
+    seprewrite_in felem_to_sizedlistarray H0.
+    rewrite felem_to_list_ws2felem in *; [|assumption].
+    ecancel_assumption.
+  Qed.
 End SpecProperties.
 
+(* FElem -> bytes for ecancel_assumption_impl. Prefer using the rewrite tactics below. *)
+#[export] Hint Extern 1 (Lift1Prop.impl1 (FElem ?px ?x) (sepclause_of_map (map.of_list_word_at ?px _))) => (rewrite felem_to_bytes; exact impl1_refl) : ecancel_impl.
 
-(* array1 -> Placeholder, only works if length sidecondition can be solved by ZnWords or lia. *)
-#[export] Hint Extern 1 (Lift1Prop.impl1 (array ptsto (word.of_Z 1) ?p ?stack) (Placeholder (field_representation:=?frep) ?p _)) => (
-    unshelve(erewrite <- (Placeholder_iff_array1 (field_representation:=frep) p _ _));
-      [ (let s := eval lazy in (felem_size_in_bytes (FieldRepresentation:=frep)) in
-          change (felem_size_in_bytes (FieldRepresentation:=frep)) with s in *; try lia; ZnWords) |
-        apply impl1_refl]) : ecancel_impl.
+(* Fail fast for non-separation logic goals. *)
+Ltac ensure_map m := lazymatch type of m with | @map.rep _ _ _ => idtac | _ => fail end.
 
-(* FElem -> Placeholder *)
-#[export] Hint Extern 1 (Lift1Prop.impl1 (FElem ?px ?x) (Placeholder ?px _)) => (apply FElem_impl_Placeholder) : ecancel_impl.
+(* Call before ecancel_assumption to recursively match and rewrite memory assumptions using the lemmas from this file.
+Applies length_tac to all side conditions.*)
+Ltac ecancel_assumption_preprocess_with length_tac :=
+  repeat match goal with
+    | |- ?G ?m => ensure_map m; match goal with H: ?P m |- _ => match P with 
+      | context[FElem ?p ?v] => match G with 
+        | context[Arrays.sizedlistarray_value _ _ p _] =>
+            seprewrite_in (felem_to_sizedlistarray p v) H
+        | context[sepclause_of_map (map.of_list_word_at p _)] =>
+            seprewrite_in (felem_to_bytes p v) H
+      end 
+      | context[Arrays.sizedlistarray_value _ _ ?p ?v] => match G with
+        | context[FElem p _] =>
+          seprewrite_in (sizedlistarray_to_felem p v) H; [length_tac |]
+      end 
+      | context[array ptsto (word.of_Z 1) ?p ?v] => match G with 
+        | context[sepclause_of_map (map.of_list_word_at p _)] =>
+            seprewrite_in (array1_iff_eq_of_list_word_at p v) H; [length_tac |]
+        | context[FElem p _] =>
+            seprewrite_in (felem_from_bytearray p v) H; [length_tac |]
+      end
+    end end
+  end.
+
+(* Rewrites FElem to bytearrays for deallocation. *)
+Ltac dealloc_preprocess :=
+    repeat match goal with
+    | |- context [anybytes ?p _ _] =>
+        match goal with
+        | H: ?P ?m |- context [map.split ?m _ _] =>
+          match P with context [FElem p ?v] =>
+            seprewrite_in (felem_to_bytearray p) H; pose proof (ws2bs_felem_length v)
+          end
+        end
+    end.
+
 
